Impl/CommitterInit.i.dfy
@@ -1,0 +1,34 @@
+include "CommitterModel.i.dfy"
+include "StateModel.i.dfy"
+
+module CommitterInit {
+  import opened CommitterModel
+  import opened StateModel
+  import opened IOModel
+
+  function PageInSuperblockReq(cm: CommitterModel, io: IO, which: uint64)
+  requires which == 0 || which == 1
+  requires io.IOInit?
+  requires cm.StatusLoadingSuperblock?
+  {
+    if which == 0 then (
+      if cm.superblock1Read.None? then (
+        var loc := Superblock1Location()
+        var (id, io') := RequestRead(io, loc);
+        var s' := cm.(superblock1Read := Some(id))
+        (s', io')
+      ) else (
+        (s, io)
+      )
+    ) else (
+      if cm.superblock2Read.None? then (
+        var loc := Superblock2Location()
+        var (id, io') := RequestRead(io, loc);
+        var s' := cm.(superblock2Read := Some(id))
+        (s', io')
+      ) else (
+        (s, io)
+      )
+    )
+  }
+}
